Wavelet/Semantics/Lts.lean
@@ -183,17 +183,6 @@ theorem Lts.Similarity.sim_step
       lts₂.Step c₂ l c₂' ∧
       hsim.Sim c₁' c₂' := hsim.choose_spec.coind
 
-theorem Lts.Similarity.refl
-  {lts : Lts C E} {c : C} :
-  Lts.Similarity lts lts c c := ⟨
-    λ c₁ c₂ => c₁ = c₂,
-    by simp,
-    by
-      intros c₁ c₂ l c₁' hc₁ hstep
-      subst hc₁
-      exists c₁'
-  ⟩
-
 theorem Lts.Similarity.refl_single
   {lts₁ lts₂ : Lts C E} {c : C}
   (single : ∀ {c l c'}, lts₁.Step c l c' → lts₂.Step c l c') :
@@ -207,12 +196,17 @@ theorem Lts.Similarity.refl_single
       simp [single hstep]
   ⟩
 
-theorem Lts.Similarity.trans
+theorem Lts.Similarity.refl
+  {lts : Lts C E} {c : C} :
+  Lts.Similarity lts lts c c := .refl_single (by simp)
+
+theorem Lts.Similarity.trans_single
   {C₁ : Type u₁} {C₂ : Type u₂} {C₃ : Type u₃} {E : Type u₄}
-  {lts₁ : Lts C₁ E} {lts₂ : Lts C₂ E} {lts₃ : Lts C₃ E}
-  {c₁ : C₁} {c₂ : C₂} {c₃ : C₃} :
+  {lts₁ : Lts C₁ E} {lts₂ lts₂' : Lts C₂ E} {lts₃ : Lts C₃ E}
+  {c₁ : C₁} {c₂ : C₂} {c₃ : C₃}
+  (single₂ : ∀ {c l c'}, lts₂.Step c l c' → lts₂'.Step c l c') :
   Lts.Similarity lts₁ lts₂ c₁ c₂ →
-  Lts.Similarity lts₂ lts₃ c₂ c₃ →
+  Lts.Similarity lts₂' lts₃ c₂ c₃ →
   Lts.Similarity lts₁ lts₃ c₁ c₃ := by
   rintro ⟨R₁₂, hsim₁₂_init, hsim₁₂_coind⟩
   rintro ⟨R₂₃, hsim₂₃_init, hsim₂₃_coind⟩
@@ -222,10 +216,18 @@ theorem Lts.Similarity.trans
   · intros c₁ c₃ l c₁' hR hstep_c₁
     have ⟨c₂, hR₁₂, hR₂₃⟩ := hR
     have ⟨c₂', hstep_c₂, hR₁₂'⟩ := hsim₁₂_coind c₁ c₂ l c₁' hR₁₂ hstep_c₁
-    have ⟨c₃', hstep_c₃, hR₂₃'⟩ := hsim₂₃_coind c₂ c₃ l c₂' hR₂₃ hstep_c₂
+    have ⟨c₃', hstep_c₃, hR₂₃'⟩ := hsim₂₃_coind c₂ c₃ l c₂' hR₂₃ (single₂ hstep_c₂)
     exists c₃'
     constructor
     · exact hstep_c₃
     · exists c₂'
+
+theorem Lts.Similarity.trans
+  {C₁ : Type u₁} {C₂ : Type u₂} {C₃ : Type u₃} {E : Type u₄}
+  {lts₁ : Lts C₁ E} {lts₂ : Lts C₂ E} {lts₃ : Lts C₃ E}
+  {c₁ : C₁} {c₂ : C₂} {c₃ : C₃} :
+  Lts.Similarity lts₁ lts₂ c₁ c₂ →
+  Lts.Similarity lts₂ lts₃ c₂ c₃ →
+  Lts.Similarity lts₁ lts₃ c₁ c₃ := .trans_single (by simp)
 
 end Wavelet.Semantics
